src/Std/Tactic/BVDecide/Bitblast/BVExpr/Circuit/Impl.lean
@@ -5,21 +5,110 @@ Authors: Henrik Böving
 -/
 prelude
 import Std.Tactic.BVDecide.Bitblast.BVExpr.Circuit.Impl.Pred
-import Std.Tactic.BVDecide.Bitblast.BoolExpr.Circuit
+
+-- TODO
 
 /-!
 This module contains the implementation of a bitblaster for general `BitVec` problems with boolean
 substructure (`BVLogicalExpr`). It is the main entrypoint into the bitblasting framework.
 -/
 
+/-!
+This module contains the logic to turn a `BoolExpr Nat` into an `AIG` with maximum subterm sharing,
+through the use of a cache that re-uses sub-circuits if possible.
+-/
+
+
 namespace Std.Tactic.BVDecide
 
-open Std.Sat
+open Std.Sat Std.Sat.AIG
 
 namespace BVLogicalExpr
 
-def bitblast (expr : BVLogicalExpr) : AIG.Entrypoint BVBit :=
-  ofBoolExprCached expr BVPred.bitblast
+def bitblast (expr : BVLogicalExpr) : Entrypoint BVBit :=
+  go AIG.empty expr |>.val
+where
+  go (aig : AIG BVBit) (expr : BVLogicalExpr) : ExtendingEntrypoint aig :=
+    match expr with
+    | .literal pred => ⟨BVPred.bitblast aig pred, by apply LawfulOperator.le_size⟩
+    | .const val => ⟨aig.mkConstCached val, (by apply LawfulOperator.le_size)⟩
+    | .not expr =>
+      let ⟨⟨aig, exprRef⟩, _⟩ := go aig expr
+      let ret := aig.mkNotCached exprRef
+      have := LawfulOperator.le_size (f := mkNotCached) aig exprRef
+      ⟨ret, by dsimp only [ret] at *; omega⟩
+    | .gate g lhs rhs =>
+      let ⟨⟨aig, lhsRef⟩, lextend⟩ := go aig lhs
+      let ⟨⟨aig, rhsRef⟩, rextend⟩ := go aig rhs
+      let lhsRef := lhsRef.cast <| by
+        dsimp only at rextend ⊢
+        omega
+      let input := ⟨lhsRef, rhsRef⟩
+      match g with
+      | .and =>
+        let ret := aig.mkAndCached input
+        have := LawfulOperator.le_size (f := mkAndCached) aig input
+        ⟨ret, by dsimp only [ret] at lextend rextend ⊢; omega⟩
+      | .xor =>
+        let ret := aig.mkXorCached input
+        have := LawfulOperator.le_size (f := mkXorCached) aig input
+        ⟨ret, by dsimp only [ret] at lextend rextend ⊢; omega⟩
+      | .beq =>
+        let ret := aig.mkBEqCached input
+        have := LawfulOperator.le_size (f := mkBEqCached) aig input
+        ⟨ret, by dsimp only [ret] at lextend rextend ⊢; omega⟩
+
+namespace bitblast
+
+theorem go_decls_size_le (expr : BVLogicalExpr) (aig : AIG BVBit) :
+    aig.decls.size ≤ (bitblast.go aig expr).val.aig.decls.size :=
+  (bitblast.go aig expr).property
+
+theorem go_decl_eq (idx) (aig : AIG BVBit) (h : idx < aig.decls.size) (hbounds) :
+    (bitblast.go aig expr).val.aig.decls[idx]'hbounds = aig.decls[idx] := by
+  induction expr generalizing aig with
+  | const =>
+    simp only [go]
+    rw [AIG.LawfulOperator.decl_eq (f := mkConstCached)]
+  | literal =>
+    simp only [go]
+    rw [AIG.LawfulOperator.decl_eq (f := BVPred.bitblast)]
+  | not expr ih =>
+    simp only [go]
+    have := go_decls_size_le expr aig
+    specialize ih aig (by omega) (by omega)
+    rw [AIG.LawfulOperator.decl_eq (f := mkNotCached)]
+    assumption
+  | gate g lhs rhs lih rih =>
+    have := go_decls_size_le lhs aig
+    have := go_decls_size_le rhs (go aig lhs).val.aig
+    specialize lih aig (by omega) (by omega)
+    specialize rih (go aig lhs).val.aig (by omega) (by omega)
+    cases g with
+    | and =>
+      simp only [go]
+      rw [AIG.LawfulOperator.decl_eq (f := mkAndCached), rih, lih]
+    | xor =>
+      simp only [go]
+      rw [AIG.LawfulOperator.decl_eq (f := mkXorCached), rih, lih]
+    | beq =>
+      simp only [go]
+      rw [AIG.LawfulOperator.decl_eq (f := mkBEqCached), rih, lih]
+
+theorem go_isPrefix_aig {aig : AIG BVBit} :
+    IsPrefix aig.decls (go aig expr).val.aig.decls := by
+  apply IsPrefix.of
+  · intro idx h
+    apply go_decl_eq
+  · apply go_decls_size_le
+
+@[simp]
+theorem go_denote_entry (entry : Entrypoint BVBit) {h} :
+    ⟦(go entry.aig expr).val.aig, ⟨entry.ref.gate, h⟩, assign⟧ = ⟦entry, assign⟧ := by
+  apply denote.eq_of_isPrefix
+  apply go_isPrefix_aig
+
+end bitblast
 
 end BVLogicalExpr
 
