src/Std/Tactic/BVDecide/Bitblast/BVExpr/Circuit/Lemmas.lean
@@ -20,18 +20,21 @@ open Std.Sat.AIG
 
 namespace BVLogicalExpr
 
-theorem bitblast.go_eval_eq_eval (expr : BVLogicalExpr) (aig : AIG BVBit) (assign : BVExpr.Assignment) :
-    ⟦ofBoolExprCached.go aig expr BVPred.bitblast, assign.toAIGAssignment⟧ = expr.eval assign := by
+namespace bitblast
+
+theorem go_eval_eq_eval (expr : BVLogicalExpr) (aig : AIG BVBit) (assign : BVExpr.Assignment) :
+    ⟦go aig expr, assign.toAIGAssignment⟧ = expr.eval assign := by
   induction expr generalizing aig with
-  | const => simp [ofBoolExprCached.go]
-  | literal => simp [ofBoolExprCached.go]
-  | not expr ih => simp [ofBoolExprCached.go, ih]
-  | gate g lhs rhs lih rih => cases g <;> simp [ofBoolExprCached.go, Gate.eval, lih, rih]
+  | const => simp [go]
+  | literal => simp [go]
+  | not expr ih => simp [go, ih]
+  | gate g lhs rhs lih rih => cases g <;> simp [go, Gate.eval, lih, rih]
+
+end bitblast
 
 theorem denote_bitblast (expr : BVLogicalExpr) (assign : BVExpr.Assignment) :
     ⟦bitblast expr, assign.toAIGAssignment⟧ = expr.eval assign := by
   unfold bitblast
-  unfold ofBoolExprCached
   rw [bitblast.go_eval_eq_eval]
 
 theorem unsat_of_bitblast (expr : BVLogicalExpr) : expr.bitblast.Unsat → expr.Unsat :=  by
