tests/lean/run/aig_optimizations.lean
@@ -1,9 +1,9 @@
-import Std.Tactic.BVDecide.Bitblast.BoolExpr
+import Std.Tactic.BVDecide.Bitblast.BVExpr
 
 open Std.Sat
 open Std.Tactic.BVDecide
 
-def mkFalseCollapsible (n : Nat) : BoolExpr Nat :=
+def mkFalseCollapsible (n : Nat) : BVLogicalExpr :=
   match n with
   | 0 => .const false
   | n + 1 =>
@@ -12,13 +12,13 @@ def mkFalseCollapsible (n : Nat) : BoolExpr Nat :=
 
 /-- info: #[Std.Sat.AIG.Decl.const false] -/
 #guard_msgs in
-#eval ofBoolExprCached (mkFalseCollapsible 1) AIG.mkAtomCached |>.aig.decls
+#eval (mkFalseCollapsible 1).bitblast.aig.decls
 
 /-- info: #[Std.Sat.AIG.Decl.const false] -/
 #guard_msgs in
-#eval ofBoolExprCached (mkFalseCollapsible 16) AIG.mkAtomCached |>.aig.decls
+#eval (mkFalseCollapsible 16).bitblast.aig.decls
 
-def mkTrueCollapsible (n : Nat) : BoolExpr Nat :=
+def mkTrueCollapsible (n : Nat) : BVLogicalExpr :=
   match n with
   | 0 => .const true
   | n + 1 =>
@@ -27,13 +27,13 @@ def mkTrueCollapsible (n : Nat) : BoolExpr Nat :=
 
 /-- info: #[Std.Sat.AIG.Decl.const true] -/
 #guard_msgs in
-#eval ofBoolExprCached (mkTrueCollapsible 1) AIG.mkAtomCached |>.aig.decls
+#eval (mkTrueCollapsible 1).bitblast.aig.decls
 
 /-- info: #[Std.Sat.AIG.Decl.const true] -/
 #guard_msgs in
-#eval ofBoolExprCached (mkTrueCollapsible 16) AIG.mkAtomCached |>.aig.decls
+#eval (mkTrueCollapsible 16).bitblast.aig.decls
 
-def mkConstantCollapsible (n : Nat) : BoolExpr Nat :=
+def mkConstantCollapsible (n : Nat) : BVLogicalExpr :=
   match n with
   | 0 => .const false
   | n + 1 =>
@@ -43,11 +43,11 @@ def mkConstantCollapsible (n : Nat) : BoolExpr Nat :=
 /-- info: (2, Std.Sat.AIG.Decl.const false) -/
 #guard_msgs in
 #eval
-  let entry := ofBoolExprCached (mkConstantCollapsible 1) AIG.mkAtomCached
+  let entry := (mkConstantCollapsible 1).bitblast
   (entry.aig.decls.size, entry.aig.decls[entry.ref.gate]!)
 
 /-- info: (2, Std.Sat.AIG.Decl.const false) -/
 #guard_msgs in
 #eval
-  let entry := ofBoolExprCached (mkConstantCollapsible 16) AIG.mkAtomCached
+  let entry := (mkConstantCollapsible 16).bitblast
   (entry.aig.decls.size, entry.aig.decls[entry.ref.gate]!)
